Iris/Iris/BI/DerivedLaws.lean
@@ -158,7 +158,7 @@ theorem imp_congr_left [BI PROP] {P P' Q : PROP} (h : P ⊣⊢ P') : (P → Q) �
 theorem imp_congr_right [BI PROP] {P Q Q' : PROP} (h : Q ⊣⊢ Q') : (P → Q) ⊣⊢ (P → Q') :=
   imp_congr .rfl h
 
-@[ne_congr, rocq_alias bi.forall_ne]
+@[ne_congr high, rocq_alias bi.forall_ne]
 theorem forall_ne [BI PROP] {Φ Ψ : α → PROP} (h : ∀ a, Φ a ≡{n}≡ Ψ a) :
     iprop(∀ a, Φ a) ≡{n}≡ iprop(∀ a, Ψ a) := sForall_ne <| by
   constructor <;> rintro _ ⟨a, rfl⟩ <;> exact ⟨_, ⟨a, rfl⟩, h _⟩
@@ -719,7 +719,7 @@ theorem pure_exists [BI PROP] {φ : α → Prop} : (∃ x, ⌜φ x⌝ : PROP) �
 /-! # Affine -/
 
 @[rocq_alias bi.affinely_ne]
-theorem affinely_ne [BI PROP] : OFE.NonExpansive (@affinely PROP _) where
+instance affinely_ne [BI PROP] : OFE.NonExpansive (@affinely PROP _) where
   ne _ _ _ h := and_ne.1 .rfl h
 #rocq_ignore bi.affinely_flip_mono' "Use _mono."
 #rocq_ignore bi.affinely_mono' "Use _mono."
@@ -852,7 +852,7 @@ instance [BIBase PROP] : Inhabited PROP where
 /-! # Absorbing -/
 
 @[rocq_alias bi.absorbingly_ne]
-theorem absorbingly_ne [BI PROP] : OFE.NonExpansive (@absorbingly PROP _) where
+instance absorbingly_ne [BI PROP] : OFE.NonExpansive (@absorbingly PROP _) where
   ne _ _ _ h := sep_ne.1 .rfl h
 #rocq_ignore bi.absorbingly_flip_mono' "Use _mono."
 #rocq_ignore bi.absorbingly_mono' "Use _mono."
@@ -1372,7 +1372,7 @@ instance absorbingly_persistent [BI PROP] (P : PROP) [Persistent P] :
 /-! # The intuitionistic modality -/
 
 @[rocq_alias bi.intuitionistically_ne]
-theorem intuitionistically_ne [BI PROP] : OFE.NonExpansive (@intuitionistically PROP _) where
+instance intuitionistically_ne [BI PROP] : OFE.NonExpansive (@intuitionistically PROP _) where
   ne _ _ _ h := affinely_ne.1 (persistently_ne.1 h)
 #rocq_ignore bi.intuitionistically_flip_mono' "Use _mono."
 #rocq_ignore bi.intuitionistically_mono' "Use _mono."
@@ -1536,7 +1536,7 @@ theorem intuitionistically_into_persistently [BI PROP] {P : PROP} [BIAffine PROP
     iprop(<affine>?true P) = iprop(<affine> P) := rfl
 
 @[rocq_alias bi.affinely_if_ne]
-theorem affinelyIf_ne {p : Bool} [BI PROP] : OFE.NonExpansive (affinelyIf (PROP := PROP) p) :=
+instance affinelyIf_ne {p : Bool} [BI PROP] : OFE.NonExpansive (affinelyIf (PROP := PROP) p) :=
   match p with
   | true => affinely_ne
   | false => OFE.id_ne
@@ -1676,7 +1676,7 @@ theorem affinelyIf_and_left_right {p : Bool} [BI PROP] {P Q : PROP} :
     iprop(<absorb>?true P) = iprop(<absorb> P) := rfl
 
 @[rocq_alias bi.absorbingly_if_ne]
-theorem absorbinglyIf_ne {p : Bool} [BI PROP] : OFE.NonExpansive (absorbinglyIf (PROP := PROP) p) :=
+instance absorbinglyIf_ne {p : Bool} [BI PROP] : OFE.NonExpansive (absorbinglyIf (PROP := PROP) p) :=
   match p with
   | true => absorbingly_ne
   | false => OFE.id_ne
@@ -1819,7 +1819,7 @@ theorem affinely_if_absorbingly_if_elim [BI PROP] {p : Bool} {P : PROP} [BIPosit
     iprop(<pers>?true P) = iprop(<pers> P) := rfl
 
 @[rocq_alias bi.persistently_if_ne]
-theorem persistentlyIf_ne {p : Bool} [BI PROP] :
+instance persistentlyIf_ne {p : Bool} [BI PROP] :
     OFE.NonExpansive (persistentlyIf (PROP := PROP) p) :=
   match p with
   | true => persistently_ne
@@ -1920,7 +1920,7 @@ theorem persistentlyIf_intutitionistically {p : Bool} [BI PROP] {P : PROP} :
 @[simp] theorem intuitionisticallyIf_true [BI PROP] (P : PROP) : iprop(□?true P) = iprop(□ P) := rfl
 
 @[rocq_alias bi.intuitionistically_if_ne]
-theorem intuitionisticallyIf_ne {p : Bool} [BI PROP] :
+instance intuitionisticallyIf_ne {p : Bool} [BI PROP] :
     OFE.NonExpansive (intuitionisticallyIf (PROP := PROP) p) :=
   match p with
   | true => intuitionistically_ne
