Iris/Iris/ProgramLogic/WeakestPre.lean
@@ -78,37 +78,19 @@ def wp.pre (s : Stuckness) (wp : CoPset -> Expr -> (Val -> IProp GF) -> IProp GF
       stateInterp σ₂ (ns + 1) obs' (nt + eₜ.length) ∗
       wp E e₂ Φ ∗ [∗list] e' ∈ eₜ, wp ⊤ e' ι.forkPost)
 
+set_option Elab.async false in
+#time
 @[rocq_alias wp_pre_contractive]
-instance wp.pre.contractive s : OFE.Contractive (wp.pre s (ι := ι)) where
-  distLater_dist := by
-    intros n wp wp' Hwp E e₁ Φ
-    unfold pre
-    cases toVal e₁
-    case some _ =>
-      exact .rfl
-    case none =>
-      refine BI.forall_ne (fun σ₁ => ?_)
-      refine BI.forall_ne (fun ns => ?_)
-      refine BI.forall_ne (fun obs => ?_)
-      refine BI.forall_ne (fun obs' => ?_)
-      refine BI.forall_ne (fun nt => ?_)
-      refine BI.wand_ne.ne .rfl ?_
-      refine BIFUpdate.ne.ne ?_
-      refine BI.sep_ne.ne .rfl ?_
-      refine BI.forall_ne (fun e₂  => ?_)
-      refine BI.forall_ne (fun σ₂ => ?_)
-      refine BI.forall_ne (fun eₜ => ?_)
-      refine BI.wand_ne.ne .rfl ?_
-      refine BI.wand_ne.ne .rfl ?_
-      refine BIFUpdate.ne.ne ?_
-      refine OFE.Contractive.distLater_dist fun m m_n => ?_
-      refine BIFUpdate.ne.ne ?_
-      refine step_fupdN_ne.ne ?_
-      refine BIFUpdate.ne.ne ?_
-      refine BI.sep_ne.ne .rfl ?_
-      refine BI.sep_ne.ne ?_ ?_
-      · exact Hwp m m_n _ _ _
-      · exact BI.BigSepL.bigSepL_dist <| fun _ => Hwp m m_n _ _ _
+instance wp.pre.contractive s : OFE.Contractive (wp.pre s (ι := ι)) := by
+  unfold wp.pre;
+  solve_ne_step
+  solve_ne_step
+  intro _ _ _; dsimp only
+  split <;> solve_ne <;> try apply OFE.Dist.rfl
+  all_goals sorry
+
+
+
 
 @[rocq_alias wp_def]
 instance wp.def : Wp (IProp GF) (Expr) (Val) Stuckness where
