Iris/Iris/Tests/Tactics.lean
@@ -2186,7 +2186,6 @@ example (P Q : PROP) :
   iintro #HPQ HQ !>
   inext
   irewrite [HPQ] at HQ
-  · exact ⟨fun _ _ _ h => affinely_ne.ne h⟩
   · iexact HQ
 
 /- Tests `irewrite` under affine and later backwards -/
@@ -2195,7 +2194,6 @@ example (P Q : PROP) :
   iintro #HPQ HQ !>
   inext
   irewrite [←HPQ] at HQ
-  · exact ⟨fun _ _ _ h => affinely_ne.ne h⟩
   · iexact HQ
 
 /- Tests `irewrite` with no matching target -/
